Pdl/Unfold.lean
@@ -24,12 +24,47 @@ def H : Program → List (List Formula × List Program)
           ).join
 | ∗α => [ (∅,ε) ] ∪ ((H α).map (fun (F,δ) => if δ = ε then [] else [(F, δ ++ [∗α])])).join
 
--- Example sanity check that associativity does not matter:
-/-
-#eval H ((?'(·2)) ;' (·1) ;' (?'(·3)))
-#eval H (( (?'(·2)) ;'   (·1) ) ;' (?'(·3)  ))
-#eval H (  (?'(·2)) ;' ( (·1)   ;' (?'(·3)) ))
--/
+open HasVocabulary
+
+theorem H_keeps_fresh α : x ∉ voc α → ∀ Fδ ∈ H α, x ∉ voc Fδ.1 ∧ x ∉ voc Fδ.2 := by
+  intro x_notin Fδ Fδ_in_H
+  cases α
+  all_goals
+    simp [H, voc,vocabOfListFormula,vocabOfListProgram,vocabOfFormula,vocabOfProgram] at *
+    subst_eqs
+  case atom_prog a =>
+    simp [vocabOfProgram]
+    assumption
+  all_goals (constructor <;> intro x x_in)
+  case sequence.left α β =>
+    rcases Fδ_in_H with ⟨l, ⟨⟨ F',δ', ⟨Fδ'_in, def_l⟩ ⟩  , Fδ_in_l⟩⟩
+    subst def_l
+    cases em (δ' = []) <;> simp_all
+    · subst_eqs
+      rw [not_or] at x_notin
+      have := H_keeps_fresh α x_notin.1 (F',[]) Fδ'_in
+      simp_all [H, voc,vocabOfListFormula,vocabOfListProgram,vocabOfFormula,vocabOfProgram]
+      apply this
+      -- take apart Fδ_in_l here???
+      sorry
+    · subst_eqs
+      rw [not_or] at x_notin
+      have := H_keeps_fresh α x_notin.1 (F',δ') Fδ'_in
+      simp_all [H, voc,vocabOfListFormula,vocabOfListProgram,vocabOfFormula,vocabOfProgram]
+  case sequence.right α β =>
+    sorry
+  case union.left α β =>
+    sorry
+  case union.right α β =>
+    sorry
+  case star.left α =>
+    sorry
+  case star.right α =>
+    sorry
+  case test.refl.left τ =>
+    sorry
+  case test.refl.right τ =>
+    sorry
 
 def Yset : (List Formula × List Program) → (Formula) → List Formula
 | ⟨F, δ⟩, φ => F ∪ [ ~ Formula.boxes δ φ ]
@@ -247,7 +282,7 @@ theorem localDiamondTruth γ ψ : (~⌈γ⌉ψ) ≡ dis ( (H γ).map (fun Fδ =>
         use w
       case inr hyp =>
         have : ∃ γ, δ = γ ++ [∗β] ∧ γ ≠ ε ∧ (Fs,γ) ∈ H β := by aesop
-        rcases this with ⟨γ, ⟨δ_def, γ_notEmpty, Fγ_in⟩⟩
+        rcases this with ⟨γ, ⟨δ_def, _, Fγ_in⟩⟩
         subst δ_def
         simp only [Yset, List.mem_union_iff, List.mem_singleton] at w_Con
         have := w_Con (~⌈⌈γ ++ [∗β]⌉⌉ψ)
@@ -369,8 +404,29 @@ theorem localDiamondTruth γ ψ : (~⌈γ⌉ψ) ≡ dis ( (H γ).map (fun Fδ =>
           (fun Fδ => if Fδ.2 = [] then Formula.bottom else Con ((~⌈⌈Fδ.2⌉⌉~·x) :: Fδ.1)) ))) =
             (dis ((H β).map (fun Fδ => if Fδ.2 = [] then Formula.bottom else Con ((~⌈⌈Fδ.2⌉⌉~ρ) :: Fδ.1))))
             := by
-          -- use that x not in β and thus also not in H β
-          sorry
+          suffices (repl_in_F x ρ (dis ((H β).map
+            (fun Fδ => if Fδ.2 = [] then Formula.bottom else Con ((~⌈⌈Fδ.2⌉⌉~·x) :: Fδ.1)) ))) =
+              ((dis ((H β).map
+                (fun Fδ => if Fδ.2 = [] then repl_in_F x ρ Formula.bottom else repl_in_F x ρ (Con ((~⌈⌈Fδ.2⌉⌉~·x) :: Fδ.1)) )))) by
+            rw [this]
+            simp only [repl_in_F, Formula.instBot]
+            -- use that x not in β and thus also not in any element of H β
+            have myFresh := H_keeps_fresh β x_not_in
+            apply listEq_to_disEq
+            rw [List.map_eq_map_iff]
+            intro Fδ Fδ_in_Hβ
+            cases em (Fδ.2 = [])
+            · simp_all
+            · simp_all only [evaluate, relate, not_forall, exists_prop, repl_in_F, Formula.instBot, Prod.forall, ite_false]
+              rw [repl_in_Con]
+              simp only [List.map_cons, repl_in_F]
+              apply listEq_to_conEq
+              simp only [List.cons.injEq, Formula.neg.injEq]
+              constructor
+              · exact repl_in_boxes_non_occ_eq _ ((myFresh _ _ (Fδ_in_Hβ)).2)
+              · exact repl_in_list_non_occ_eq _ ((myFresh _ _ (Fδ_in_Hβ)).1)
+          -- remains to push repl_in_F through dis and map
+          exact repl_in_disMap x ρ (H β) (fun Fδ => Fδ.2 = []) (fun Fδ => (Con ((~⌈⌈Fδ.2⌉⌉~·x) :: Fδ.1)))
         rw [this, disEval, helper]
         clear this
         rintro ⟨⟨Fs,δ⟩, ⟨Fδ_in, repl_w_⟩⟩
@@ -514,7 +570,7 @@ theorem existsDiamondH (v_γ_w : relate M γ v w) :
       use ⟨∅, ε⟩
       simp [H, relateSeq]
     case inr hyp =>
-      rcases hyp with ⟨v_neq_w, ⟨v1, v_neq_v1, v_β_v1, v1_βS_w⟩⟩
+      rcases hyp with ⟨_, ⟨v1, v_neq_v1, v_β_v1, v1_βS_w⟩⟩
       have IHβ := existsDiamondH v_β_v1
       rcases IHβ with ⟨⟨Fs,δ⟩, Fδ_in, v_Fs, v_δ_v1⟩
       use ⟨Fs, δ ++ [∗β]⟩
